\documentclass[nooutcomes]{ximera}
\usepackage{booktabs}
%% handout
%% space
%% newpage
%% numbers
%% nooutcomes

\renewcommand{\outcome}[1]{\marginpar{\null\vspace{2ex}\scriptsize\framebox{\parbox{0.75in}{\begin{raggedright}P\arabic{problem} Outcome: #1\end{raggedright}}}}}

\renewenvironment{freeResponse}{
\ifhandout\setbox0\vbox\bgroup\else
\begin{trivlist}\item[\hskip \labelsep\bfseries Solution:\hspace{2ex}]
\fi}
{\ifhandout\egroup\else
\end{trivlist}
\fi}

\newcommand{\RR}{\mathbb R}
\renewcommand{\d}{\,d}
\newcommand{\dd}[2][]{\frac{d #1}{d #2}}
\renewcommand{\l}{\ell}
\newcommand{\ddx}{\frac{d}{dx}}
\everymath{\displaystyle}
\newcommand{\dfn}{\textbf}
\newcommand{\eval}[1]{\bigg[ #1 \bigg]}


\title{Breakout Session 25 Solutions}

\begin{document}
\begin{abstract}
  % \textbf{A look back:} In a previous (April 14, 2016) Breakout Session you practiced applying a few basic properties of integrals and the mbean value theorem for integrals.
  %
  % \textbf{Overview:} In today's (April 19, 2016) Breakout Session you'll practice applying one of the most important techniques for evaluating (definite and indefinite) integrals: substitution.
  %
  % \textbf{A look ahead:} In the next (April 21, 2016) Breakout Session you'll learn how definite integrals are used to compute net change.
\end{abstract}
\maketitle

% \section{Learning Outcomes}
% \label{section:learning-outcomes}
% The following outcomes are \emph{not an exhaustive} list of the skills you will need to develop and integrate for demonstration on quizzes and exams.
% This list is meant to be a starting point for conversation (with your Lecturer, Breakout Session Instructor, and fellow learners) for organizing your knowledge and monitoring the development of your skills.
%
% \begin{itemize}
%   \item
%     Calculate indefinite integrals (antiderivatives) using u-substitution.
%   \item
%     Calculate definite integrals using u-substitution
%   \item
%     Practice until you are familiar with a lot of patterns.
%   \item
%     Undo the Chain Rule.
%   \item
%     Evaluate definite and indefinite integrals through a change of variables.
% \end{itemize}
% \newpage

\section{Substitution Rule for Indefinite Integrals}
\begin{problem}
  \outcome{Calculate indefinite integrals (antiderivatives) using u-substitution.}
  \outcome{Practice until you are familiar with a lot of patterns.}
  What are two substitutions that can be used to evaluate the integral \begin{equation*} \int x \sqrt{x+8} \d x \end{equation*}
	\begin{freeResponse}
    Two substitutions which work are $u=x+8$ and $v=\sqrt{x+8}$.
    I find the $u=x+8$ to be the more ``obvious" solution, so	let us work through that one first.
    \begin{equation*}
      u=x+8 \quad \Longrightarrow \quad \d u = \d x \quad \text{and} \quad x = u-8
		\end{equation*}
    Substituting into the original integral and solving:
		\begin{align*}
      \int x \sqrt{x+8} \d x
      &= \int (u-8) \sqrt{u} \d u  \\
      &= \int (u^{\frac{3}{2}} - 8u^{\frac{1}{2}} ) \d u  \\
      &= \frac{2}{5} u^{\frac{5}{2}} - 8 \cdot \frac{2}{3} u^{\frac{3}{2}} + C  \\
      &= \frac{2}{5}(x+8)^{\frac{5}{2}} - \frac{16}{3} (x+8)^{\frac{3}{2}} + C
    \end{align*}

    To the other solution, letting $v=\sqrt{x+8}$ gives:
    \begin{equation*}
      \d v = \frac{1}{2 \sqrt{x+8}} \d x = \frac{1}{2v} \d x 	\quad	\Longrightarrow \quad \d x = 2v \d v
    \end{equation*}
    and
    \begin{equation*}
       v = \sqrt{x+8} \quad \Longrightarrow \quad v^2 = x+8 \quad \Longrightarrow \quad x= v^2-8
    \end{equation*}

     Substituting into the original integral and solving:
    \begin{align*}
       \int x \sqrt{x+8} \d x
       &= \int (v^2-8)(v)(2v)\d v  \\
       &= \int (2v^4 - 16v^2) \d v  \\
       &= \frac{2}{5} v^5 - \frac{16}{3} v^3  \\
       &= \frac{2}{5}(\sqrt{x+8})^5 - \frac{16}{3} (\sqrt{x+8})^3
    \end{align*}
  \end{freeResponse}
\end{problem}

\begin{problem}
  \outcome{Calculate indefinite integrals (antiderivatives) using u-substitution.}
  \outcome{Undo the Chain Rule.}
Compute the  integral: $\int \cos(x) \sqrt{\sin(x)} \d x$
  \begin{freeResponse}
		Let $v = \sin(x)$.  Then $\d v = \cos(x) \d x$, and so
		\begin{align*}
			\int \cos(x) \sqrt{\sin(x)} \d x &= \int \sqrt{v} \d v  \\
			&= \frac{2}{3} v^{\frac{3}{2}} + C  \\
			&= \frac{2}{3} (\sin(x))^{\frac{3}{2}} + C.
		\end{align*}
	\end{freeResponse}
\end{problem}

\begin{problem}
  \outcome{Calculate indefinite integrals (antiderivatives) using u-substitution.}
  \outcome{Practice until you are familiar with a lot of patterns.}
Compute the integral $\int \frac{x}{\sqrt{x-4}} \d x$
	\begin{freeResponse}
    Let $u = \sqrt{x - 4}$.
    Then
    \begin{align*}
      du = \frac{dx}{2\sqrt{x-4}}
      &\implies 2du = \frac{dx}{\sqrt{x-4}}
    \end{align*}
    and
    \begin{align*}
      u = \sqrt{x - 4}
      &\implies x = u^2 +4.
    \end{align*}

    Therefore
    \begin{align*}
      \int \frac{x}{\sqrt{x-4}} \d x
      &= \int 2(u^2 + 4) \d u \\
      &= 2\left(\frac{u^3}{3} + 4u \right) + C\\
      &= 2\left(\frac{(\sqrt{x-4})^3}{3} + 4\sqrt{x-4}\right)
    \end{align*}
	\end{freeResponse}
\end{problem}

\begin{problem}
  \outcome{Calculate indefinite integrals (antiderivatives) using u-substitution.}
  \outcome{Practice until you are familiar with a lot of patterns.}
Compute the integral $ \int \frac{1+3x}{4+4x^2} \d x$
  \begin{freeResponse}
		First notice that
		\begin{equation*}
			\int \frac{1+3x}{4+4x^2} \d x = \frac{1}{4} \int \frac{1+3x}{1+x^2} \d x = \frac{1}{4} \int \left( \frac{1}{1+x^2} + \frac{3x}{1+x^2} \right) \d x.
		\end{equation*}
		The first integral is $\arctan(x)$, and so we have
		\begin{equation}\label{3b1}
			\int \frac{1+3x}{4+4x^2} \d x = \frac{1}{4} \arctan(x) + \frac{3}{4} \int \frac{x}{1+x^2} \d x.
		\end{equation}
		We can solve this second integral by substitution.
    Let $u=1+x^2$.
    Then $\d u = 2x \d x$ and $\frac{1}{2} \d u = x \d x$.
    So
		\begin{equation}\label{3b2}
			\int \frac{x}{1+x^2} \d x = \frac{1}{2} \int \frac{1}{u} \d u = \frac{1}{2} \ln|u| +C = \frac{1}{2} \ln(1+x^2) + C.
		\end{equation}
		Plugging equation \eqref{3b2} into equation \eqref{3b1} yields
		\begin{equation*}
			\int \frac{1+3x}{4+4x^2} \d x = \frac{1}{4} \arctan(x) + \frac{3}{8} \ln(1+x^2) + C.
		\end{equation*}
	\end{freeResponse}
\end{problem}

\section{Substitution Rule for Definite Integrals}
\begin{problem}
Evaluate the following integrals:

	\begin{enumerate}
    \outcome{Calculate definite integrals using u-substitution}
    \outcome{Undo the Chain Rule.}
	\item  $\int_{-2}^1 t^2 \sin(t^3) \d t$
		\begin{freeResponse}
		Let $u=u(t) = t^3$, where $``u(t)"$ is just meant to indicate that the variable $u$ is really a function of $t$.  Then $\d u = 3t^2 \d t$.  But also notice that
			\begin{align*}
			u(-2) &= (-2)^3 = -8  \\
			u(1) &= 1^3 = 1
			\end{align*}
		Then
			\begin{align*}
			\int_{-2}^1 t^2 \sin(t^3) \d t &= \frac{1}{3} \int_{-2}^1 3 t^2 \sin(t^3) \d t  \\
			&= \frac{1}{3} \int_{-8}^1 \sin(u) \d u  \\
			&= - \frac{1}{3} \eval{\cos(u)}_{-8}^1  \\
			&= - \frac{1}{3} ( \cos(1) - \cos(-8)).
			\end{align*}
		\end{freeResponse}

	\item  $\int_0^{\frac{1}{2}} \frac{13e^x}{3e^x - 5} \d x$
  \outcome{Calculate definite integrals using u-substitution}
		\begin{freeResponse}
		Let $v=3e^x - 5$.  Then
			\begin{align*}
			&\d v = 3e^x \d x  \\
			&v(0) = 3e^0 -5= 3-5=-2  \\
			&v\left( \frac{1}{2} \right) = 3e^{\frac{1}{2}} - 5.
			\end{align*}
		So
			\begin{align*}
			\int_0^{\frac{1}{2}} \frac{13e^x}{3e^x - 5} \d x &= \frac{13}{3} \int_0^{\frac{1}{2}} \frac{3e^x}{3e^x - 5} \d x  \\
			&= \frac{13}{3} \int_{-2}^{3e^{\frac{1}{2}}-5} \frac{1}{v} \d v  \\
			&= \frac{13}{3} \eval{\ln|v|}_{-2}^{3e^{\frac{1}{2}}-5}  \\
			&= \frac{13}{3} \left( \ln|3e^{\frac{1}{2}}-5| - \ln|-2| \right).  \\
			\end{align*}
		\end{freeResponse}
	\end{enumerate}
\end{problem}

\begin{problem}
Evaluate the following integrals:

	\begin{enumerate}
    \item $\int_0^{\pi/2} \frac{\cos(x)}{4 + \sin(x)} \d x$
    \outcome{Calculate definite integrals using u-substitution}
    \outcome{Undo the Chain Rule.}
    \begin{freeResponse}
      Let $u = 4 + \sin(x)$.
      Then
      \begin{align*}
        u = 4 + \sin(x) \implies du = \cos(x) dx
      \end{align*}
      and
      \begin{align*}
       \int_0^{\pi/2} \frac{\cos(x)}{4 + \sin(x)} \d x
       &= \int_{x = 0}^{x = \pi/2} \frac{du}{u} \\
       &= \int_{4}^{5} \frac{du}{u}\\
       &= \eval{\ln|u|}_4^5 = \ln(5) - \ln(4)
      \end{align*}
    \end{freeResponse}
	\item  $\int_1^4 \frac{e^{\sqrt{x}}}{3\sqrt{x}} \d x$
    \outcome{Calculate definite integrals using u-substitution}
		\begin{freeResponse}
		Let $w=\sqrt{x}$.  Then
			\begin{align*}
			&\d w = \frac{1}{2 \sqrt{x}} \d x  \\
			&w(1) = \sqrt{1} = 1  \\
			&w(4) = \sqrt{4} = 2.
			\end{align*}
		So
			\begin{align*}
			\int_1^4 \frac{e^{\sqrt{x}}}{3\sqrt{x}} \d x &= \frac{2}{3} \int_1^4 \frac{e^{\sqrt{x}}}{2\sqrt{x}} \d x  \\
			&= \frac{2}{3} \int_1^2 e^w \d w  \\
			&= \frac{2}{3} \eval{e^w}_1^2  \\
			&= \frac{2}{3} (e^2 - e).
			\end{align*}
		\end{freeResponse}

	\item  $\int_{\frac{\pi}{3}}^{\frac{\pi}{2}} \sin(x) \sec^2(\cos(x)) \d x$
		\begin{freeResponse}
		Let $u=\cos(x)$.  Then
			\begin{align*}
			&\d u = -\sin(x) \d x  \\
			&u\left( \frac{\pi}{3} \right) = \frac{1}{2}  \\
			&u\left( \frac{\pi}{2} \right) = 0.
			\end{align*}
		So
			\begin{align*}
			\int_{\frac{\pi}{3}}^{\frac{\pi}{2}} \sin(x) \sec^2(\cos(x)) \d x &= - \int_{\frac{1}{2}}^0 \sec^2(u) \d u   \\
			&= - \eval{\tan(u)}_{\frac{1}{2}}^0  \\
			&=  -\left( 0 - \tan\left( \frac{1}{2} \right) \right)  \\
			&= \tan \left( \frac{1}{2} \right).
			\end{align*}
		\end{freeResponse}
	\end{enumerate}
\end{problem}

\section{Extra Problems for Personal Practice}
\begin{problem}
Compute the integral $\int \sec^2(x) \tan(x) \d x$
	\begin{freeResponse}
		Let $u = \tan(x)$.  Then $\d u = \sec^2 (x) \d x$, and so
		\begin{align*}
			\int \sec^2(x) \tan(x) \d x &= \int u \d u  \\
			&= \frac{1}{2} u^2 + C  \\
			&= \frac{1}{2} \tan^2(x) + C.
		\end{align*}
	   Note that the substitution $v=\sec(x)$ would also work to solve this problem.
		It is a good exercise to work this out!
	\end{freeResponse}
\end{problem}

\begin{problem}
Evaluate the following integrals:
	\begin{enumerate}
	\item  $\int \frac{13x^7}{\sqrt{3x^4-5}} \d x$
		\begin{freeResponse}
		Let $v = 3x^4 - 5$.  Then
			\begin{align*}
			&\d v = 12 x^3 \d x  \\
			&x^4 = \frac{1}{3} (v + 5).
			\end{align*}
		So
			\begin{align*}
			\int \frac{13x^7}{\sqrt{3x^4-5}} \d x &= \frac{13}{12} \int \frac{(x^4)(12 x^3)}{\sqrt{3x^4-5}} \d x  \\
			&= \frac{13}{12} \int \frac{\frac{1}{3} (v+5)}{\sqrt{v}} \d v  \\
			&= \frac{13}{36} \int \left( v^{\frac{1}{2}} + 5v^{-\frac{1}{2}} \right) \d v  \\
			&= \frac{13}{36} \left( \frac{2}{3} v^{\frac{3}{2}} + 10 v^{\frac{1}{2}} \right) + C  \\
			&= \frac{13}{54} (3x^4-5)^{\frac{3}{2}} + \frac{65}{18} \sqrt{3x^4 - 5} + C.
			\end{align*}
		\end{freeResponse}

	\item  $\int \frac{x^3}{x^2 - 3} \d x$
		\begin{freeResponse}
		Let $w = x^2 - 3$.  Then
			\begin{align*}
			&\d w = 2x \d x  \\
			&x^2 = w + 3.
			\end{align*}
		So
			\begin{align*}
			\int \frac{x^3}{x^2 - 3} \d x &= \frac{1}{2} \int \frac{(x^2)(2x)}{x^2 - 3} \d x  \\
			&= \frac{1}{2} \int \frac{w+3}{w} \d w  \\
			&= \frac{1}{2} \int \left(1 + \frac{3}{w} \right) \d w  \\
			&= \frac{1}{2} \left( w + 3 \ln|w| \right) + C  \\
			&= \frac{1}{2} \left( x^2 - 3 + 3\ln|x^2-3| \right) + C.
			\end{align*}
		\end{freeResponse}
	\end{enumerate}
\end{problem}

\begin{problem}
  $\int \left( 3t^2 - 4 + \frac{1}{t} \right) e^{t^3 - 4t + \ln(t) -
    9} \d t$
  \begin{freeResponse}
    This problem looks a lot more difficult than it really is.
    Let $w=t^3 - 4t + \ln(t) - 9$.
    Then $\d w = \left( 3t^2 - 4 + \frac{1}{t} \right) \d t$.
    But this is exactly the coefficient of the exponential term in the integral.
    So
    \begin{align*}
      \int \left( 3t^2 - 4 + \frac{1}{t} \right) e^{t^3 - 4t + \ln(t) - 9} \d t &= \int e^w \d w  \\                                                                           &= e^w + C  \\                                                                                &= e^{t^3 - 4t + \ln(t) - 9} + C.
    \end{align*}
  \end{freeResponse}
\end{problem}

\begin{problem}
$\int 2t \sin \left( t^2 \right) \d t$
  \begin{freeResponse}
    Let $w=t^2$.  Then $\d w = 2t \d t$, and so
    \begin{align*}
      \int 2t \sin(t^2) \d t &= \int \sin(w) \d w  \\
                             &= - \cos(w) + C  \\
                             &= - \cos(t^2) + C.
    \end{align*}
  \end{freeResponse}
\end{problem}

\begin{problem}
  $\int \frac{x^2 }{1 + x^2} \d x$
  \begin{freeResponse}
    In general, when integrating a rational function where the degree of the numerator is greater than or equal to the degree of the denominator, you want to do long division to get the smallest possible degree in the numerator.
    But watch this slick little trick:
    \begin{equation*}
      \frac{x^2}{1+x^2} = \frac{1 + x^2 - 1}{1+x^2} = \frac{1+x^2}{1+x^2} - \frac{1}{1+x^2} = 1 - \frac{1}{1+x^2}.
    \end{equation*}
    So
    \begin{align*}
      \int \frac{x^2 }{1 + x^2} \d x &= \int \left( 1 - \frac{1}{1+x^2} \right) \d x  \\                                     &= x - \arctan(x) + C.
    \end{align*}
    I learned the trick above through tons and tons of practice solving integrals.
    So guess what is a good idea for you to do before the final exam???
  \end{freeResponse}
\end{problem}

\begin{problem}
Find the error in the following ``solution":

Find $\int_{-2}^2 \frac{1}{x^8 - 1} \d x$

	\begin{image}
	\includegraphics[trim= 120 320 350 180]{Images/Figure1.pdf}
	\end{image}

	\begin{freeResponse}
	The error is that the function $\frac{1}{x^8-1}$ is not defined at $x=1$, and is therefore not continuous on the interval $[-2,2]$.
	\end{freeResponse}
\end{problem}
\end{document}
%
