\documentclass[nooutcomes]{ximera}
%% handout
%% space
%% newpage
%% numbers
%% nooutcomes


\input{../preamble.tex} %% we can turn off input when making a master document

\title{3.4 The Product and Quotient Rules (Solutions)}  

\begin{document}
\begin{abstract}		\end{abstract}
\maketitle

\section*{Warm up:} 
Differentiate the function $f(x) = \frac{1}{x^8}$ two different ways.

	\begin{freeResponse}
	First way:  Since $f(x) = \frac{1}{x^8} = x^{-8}$, $f'(x) = -8x^{-8-1} = -8x^{-9} = -\frac{8}{x^9}$.
	
	Second way:  Using the quotient rule, 
	$f'(x) = \frac{(x^8 \cdot \ddx(1)) - (1 \cdot \ddx(x^8))}{(x^8)^2}
	= \frac{(x^8 \cdot 0) - (1 \cdot 8x^7)}{x^{16}}
	= \frac{-8x^7}{x^{16}}
	= - \frac{8}{x^9}$.
	\end{freeResponse}	
	
	
	
	
	

\section*{Group work:}

%problem 1
\begin{problem}
Differentiate the following functions:

	\begin{enumerate}
	
	%part a
	\item  $f(x) = (x^2 + 4x - 7) e^{-2x}$
			\begin{freeResponse}
			$f'(x) = \left( \ddx(x^2 + 4x - 7) \cdot e^{-2x} \right) + \left((x^2 + 4x - 7) \cdot \ddx(e^{-2x}) \right)
			= ((2x+4)(e^{-2x}) + (x^2 + 4x - 7)(-2e^{-2x})
			= (2x + 4 - 2x^2 - 8x + 14)e^{-2x}
			= (-2x^2 - 6x + 18)e^{-2x}$.
			\end{freeResponse}
			
			
			
	%part b
	\item  $g(x) = \frac{x^2 + 4x - 7}{e^{-2x}}$
			\begin{freeResponse}
			$g'(x) = \frac{\left( e^{-2x} \cdot \ddx(x^2 + 4x - 7) \right) - \left( (x^2 + 4x - 7) \cdot \ddx(e^{-2x}) \right)}{(e^{-2x})^2}
			= \frac{((e^{-2x}) \cdot (2x+4)) - ((x^2 + 4x - 7) \cdot (-2e^{-2x}))}{e^{-4x}}
			= \frac{(2x + 4 + 2x^2 + 8x - 14)e^{-2x}}{e^{-4x}}
			= \frac{2x^2 + 10x - 10}{e^{-2x}}$.
			\end{freeResponse}
			
			
			
			
	\end{enumerate}		
\end{problem}
	
	
	
	
			
			

%problem 2			
\begin{problem}
Suppose that $f(5) = 7$, $f'(5) = 8$, $g(5) = 3$, and $g'(5) = -4$.  Find:

	\begin{enumerate}
	
	%part a
	\item  $(fg)'(5)$.
		\begin{freeResponse}
		$(fg)'(5) = (f'(5) \cdot g(5)) + (f(5) \cdot g'(5))
		= (8)(3) + (7)(-4)
		= 24 - 28 = -4$.
		\end{freeResponse}
		
		
		
	%part b
	\item $ \left( \frac{f}{g} \right)' (5)$
		\begin{freeResponse}
		$ \left( \frac{f}{g} \right)' (5)
		= \frac{(g(5) \cdot f'(5)) - (f(5) \cdot g'(5))}{(g(5))^2}
		= \frac{(3)(8) - (7)(-4)}{3^2}
		= \frac{24 + 28}{9}
		= \frac{52}{9}$.
		\end{freeResponse}
		
		
		
	%part c
	\item $ \left( \frac{g}{f} \right)' (5)$
		\begin{freeResponse}
		$\left( \frac{g}{f} \right)' (5)
		= \frac{(f(5) \cdot g'(5)) - (g(5) \cdot f'(5))}{(f(5))^2}
		= \frac{(7)(-4) - (3)(8)}{7^2}
		= \frac{-28 - 24}{49}
		= - \frac{52}{49}$.
		\end{freeResponse}
		
	
	
	\end{enumerate}
		
\end{problem}









%problem 3			
\begin{problem}
Find the following derivatives:
	\begin{enumerate}
	
	%part a
	\item  Given $g(x) = x^3 f(x)$, $f(2) = 4$, and $f'(2) = 7$, find the equation of the tangent line to the graph of $g(x)$ at $x=2$.
		\begin{freeResponse}
		$g'(x) = 3x^2 f(x) + x^3 f'(x)$.  So $g'(2) = 12$
		\end{freeResponse}
		
		
		
	%part b
	\item  Given that $h(x) = \frac{x f(x)}{x-3}$, $f(2) = 4$, and $f'(2) = 7$, find the equation of the tangent line to the graph of $h(x)$ at $x=2$.  
		\begin{freeResponse}
		
		\end{freeResponse}
		
		
		
	%part c
	\item  Given the following table, find $\ddx \left( \frac{f(x)}{e^x g(x)} \right)$ at $x=2$. 
	
	$\begin{array}{|c|c|c|c|c|c|}
	\hline
	x	&	1	&	2	&	3	&	4	&	5	\\
	\hline
	f(x)	&	5	&	3	&	0	&	-4	&	3	\\
	\hline
	f'(x)	&	-3	&	-5	&	-2	&	6	&	-4	\\
	\hline
	g(x)	&	6	&	9	&	-8	&	13	&	15	\\
	\hline
	g'(x)	&	8	&	5	&	-10	&	7	&	6	\\
	\hline
	\end{array}$
	
	 
		\begin{freeResponse}
		
		\end{freeResponse}
		
		
		
	\end{enumerate}
		
\end{problem}







	
	
	
	
	
	
	
	
	

	










								
				
				
	














\end{document} 


















